src/exp/semantics.lean
@@ -1,0 +1,29 @@
+import .lc
+import .subst_open
+import tactics
+
+namespace tts ------------------------------------------------------------------
+namespace exp ------------------------------------------------------------------
+variables {V : Type} -- Type of variable names
+variables {e₁ e₂ : exp V} -- Expressions
+
+theorem lc_value : ∀ {e : exp V}, e.value → e.lc
+  | _ (value.lam p) := lc_lam.mpr p
+
+theorem lc_red_left (h : red e₁ e₂) : e₁.lc :=
+  by induction h; simp [and.assoc] at *; note_all_applied lc_value; tauto
+
+variables [decidable_eq V] [finset.has_fresh V]
+
+theorem lc_red_right (h : red e₁ e₂) : e₂.lc :=
+  begin
+    induction h,
+    case red.app₁ { simp at *, tauto },
+    case red.app₂ { simp at *, note_all_applied lc_value, tauto },
+    case red.lam : _ _ lc_eb val_ea { exact lc_open lc_eb (lc_value val_ea) },
+    case red.let₁ { simp at *, tauto },
+    case red.let₂ : _ _ val_ed lc_eb { exact lc_open lc_eb (lc_value val_ed) }
+  end
+
+end /- namespace -/ exp --------------------------------------------------------
+end /- namespace -/ tts --------------------------------------------------------
