src/tactics.lean
@@ -1,0 +1,27 @@
+import meta.expr
+import tactic.basic
+
+meta def name.update_suffix : name → (string → string) → name
+| name.anonymous        _ := name.anonymous
+| (name.mk_string s p)  f := name.mk_string (f s) p
+| (name.mk_numeral n p) _ := name.mk_numeral n p
+
+namespace tactic ---------------------------------------------------------------
+namespace interactive ----------------------------------------------------------
+
+open interactive
+open interactive.types
+
+meta def note_all_applied (p : parse texpr) : tactic unit :=
+  do e ← to_expr p,
+     et ← infer_type e,
+     guard et.is_pi <|> fail format!"'note_all_applied' expects a function, got '{et}'",
+     ctx ← local_context,
+     ctx.for_each $ λ h, do
+       ht ← infer_type h,
+       tactic.try $ do
+         unify ht et.binding_domain,
+         note (h.local_pp_name.update_suffix (++ "'")) none (e.mk_app [h])
+
+end /- namespace -/ interactive ------------------------------------------------
+end /- namespace -/ tactic -----------------------------------------------------
